upd: renaming bitfield extract and insert; add: some proofs for encoding proof

theory/rBPFCommType.thy
@@ -79,11 +79,11 @@ definition arsh32 :: "i32 \<Rightarrow> nat \<Rightarrow> i32" where
 definition arsh64 :: "i64 \<Rightarrow> nat \<Rightarrow> i64" where
 "arsh64 x n = (if bit x 63 then or (drop_bit n x) (((2^n) -1) << 64-n) else drop_bit n x)"
 
-definition unsigned_bitfield_extract_u8 :: "nat \<Rightarrow> nat \<Rightarrow> u8 \<Rightarrow> u8" where
-"unsigned_bitfield_extract_u8 pos width n = and ((2 ^ width) - 1) (n >> pos)"
+definition bitfield_extract :: "nat \<Rightarrow> nat \<Rightarrow> ('a :: len word) \<Rightarrow> ('a :: len word)" where
+"bitfield_extract pos width n = and ((2 ^ width) - 1) (n >> pos)"
 
-definition bitfield_insert_u8 :: "nat \<Rightarrow> nat \<Rightarrow> u8 \<Rightarrow> u8 \<Rightarrow> u8" where                                                      
-"bitfield_insert_u8 pos width n p = (
+definition bitfield_insert :: "nat \<Rightarrow> nat \<Rightarrow> ('a :: len word) \<Rightarrow> ('a :: len word) \<Rightarrow> ('a :: len word)" where
+"bitfield_insert pos width n p = (
   let mask = ((2 ^ width) - 1) << pos in
     or ((and ((2 ^ width) - 1) p) << pos)
        (and n (not mask))
