theory/x64Disassembler.thy
@@ -13,14 +13,14 @@ value "[(1::nat)]!(1::nat)" returns an error, we should have a nth_error? *)
 definition x64_decode_op_0x66 :: "nat \<Rightarrow> x64_bin \<Rightarrow> (nat * instruction) option" where
 "x64_decode_op_0x66 pc l_bin = (
   case nth_error l_bin (pc+1) of None \<Rightarrow> None | Some h1 \<Rightarrow>
-    if unsigned_bitfield_extract_u8 4 4 h1 \<noteq> 0b0100 then  
+    if bitfield_extract 4 4 h1 \<noteq> 0b0100 then  
       \<comment> \<open> R7.1 [legacy + opcode + modrm + imm] \<close>
       case nth_error l_bin (pc+2) of None \<Rightarrow> None | Some reg \<Rightarrow>
-      let modrm = unsigned_bitfield_extract_u8 6 2 reg in
-      let reg1  = unsigned_bitfield_extract_u8 3 3 reg in
-      let reg2  = unsigned_bitfield_extract_u8 0 3 reg in
-      let src   = bitfield_insert_u8 3 1 reg1 0 in
-      let dst   = bitfield_insert_u8 3 1 reg2 0 in
+      let modrm = bitfield_extract 6 2 reg in
+      let reg1  = bitfield_extract 3 3 reg in
+      let reg2  = bitfield_extract 0 3 reg in
+      let src   = bitfield_insert 3 1 reg1 0 in
+      let dst   = bitfield_insert 3 1 reg2 0 in
         if h1 = 0xc1 then 
        \<comment> \<open> P2887 `ROL : register by immediate count` -> `0x66 1100 000w : 11 000 reg : imm8` \<close>
           case nth_error l_bin (pc+3) of None \<Rightarrow> None | Some imm \<Rightarrow>
@@ -51,17 +51,17 @@ definition x64_decode_op_0x66 :: "nat \<Rightarrow> x64_bin \<Rightarrow> (nat *
             else None
         else None
     else  
-      let w = unsigned_bitfield_extract_u8 3 1 h1 in
-      let r = unsigned_bitfield_extract_u8 2 1 h1 in
-      let x = unsigned_bitfield_extract_u8 1 1 h1 in
-      let b = unsigned_bitfield_extract_u8 0 1 h1 in (
+      let w = bitfield_extract 3 1 h1 in
+      let r = bitfield_extract 2 1 h1 in
+      let x = bitfield_extract 1 1 h1 in
+      let b = bitfield_extract 0 1 h1 in (
         case nth_error l_bin (pc+2) of None \<Rightarrow> None | Some op \<Rightarrow> (
         case nth_error l_bin (pc+3) of None \<Rightarrow> None | Some reg \<Rightarrow> (
-        let modrm = unsigned_bitfield_extract_u8 6 2 reg in
-        let reg1  = unsigned_bitfield_extract_u8 3 3 reg in
-        let reg2  = unsigned_bitfield_extract_u8 0 3 reg in
-        let src   = bitfield_insert_u8 3 1 reg1 r in
-        let dst   = bitfield_insert_u8 3 1 reg2 b in
+        let modrm = bitfield_extract 6 2 reg in
+        let reg1  = bitfield_extract 3 3 reg in
+        let reg2  = bitfield_extract 0 3 reg in
+        let src   = bitfield_insert 3 1 reg1 r in
+        let dst   = bitfield_insert 3 1 reg2 b in
           \<comment> \<open> R7.3 [legacy + rex + opcode + modrm + imm] \<close>
           if op = 0xc1 then 
           \<comment> \<open> P2887 `ROL : register by immediate count` -> `0x66 1100 000w : 11 000 reg : imm8` \<close>
@@ -105,21 +105,21 @@ definition x64_decode_op_0x0f :: "nat \<Rightarrow> x64_bin \<Rightarrow> (nat *
     if op = 0x31 then 
       Some (2, Prdtsc)
     \<comment> \<open> P2877 `BSWAP: register `   -> `0000 1111 : 1100 1 reg` \<close>
-    else if unsigned_bitfield_extract_u8 3 5 op = 0b11001 then
-      let reg2 = unsigned_bitfield_extract_u8 0 3 op in
-      let dst  = bitfield_insert_u8 3 1 reg2 0 in
+    else if bitfield_extract 3 5 op = 0b11001 then
+      let reg2 = bitfield_extract 0 3 op in
+      let dst  = bitfield_insert 3 1 reg2 0 in
         case ireg_of_u8 dst of None \<Rightarrow> None | Some dst \<Rightarrow> (
           Some (2, Pbswapl dst))
     \<comment> \<open> R8.2 [escape + opcode + modrm] \<close>
     \<comment> \<open> P2919 `MOVcc : resgister2  to resgister1 ` -> `0100 0R0B 0000 1111: 0100 tttn : 11 reg1 reg2` \<close>
-    else if unsigned_bitfield_extract_u8 4 4 op = 0b0100 then
-      let flag = (unsigned_bitfield_extract_u8 0 4 op) in 
+    else if bitfield_extract 4 4 op = 0b0100 then
+      let flag = (bitfield_extract 0 4 op) in 
       case nth_error l_bin (pc+2) of None \<Rightarrow> None | Some reg \<Rightarrow>
-      let modrm = unsigned_bitfield_extract_u8 6 2 reg in
-      let reg1  = unsigned_bitfield_extract_u8 3 3 reg in
-      let reg2  = unsigned_bitfield_extract_u8 0 3 reg in
-      let src   = bitfield_insert_u8 3 1 reg1 0 in
-      let dst   = bitfield_insert_u8 3 1 reg2 0 in
+      let modrm = bitfield_extract 6 2 reg in
+      let reg1  = bitfield_extract 3 3 reg in
+      let reg2  = bitfield_extract 0 3 reg in
+      let src   = bitfield_insert 3 1 reg1 0 in
+      let dst   = bitfield_insert 3 1 reg2 0 in
         if modrm = 0b11 then
           case cond_of_u8 flag of None \<Rightarrow> None | Some t \<Rightarrow>(
           case ireg_of_u8 src of None \<Rightarrow> None | Some src \<Rightarrow> (
@@ -128,8 +128,8 @@ definition x64_decode_op_0x0f :: "nat \<Rightarrow> x64_bin \<Rightarrow> (nat *
         else None
     \<comment> \<open> R8.3 [escape + opcode + displacement] \<close>
     \<comment> \<open> P2880 `JCC: full displacement` -> `0000 1111 : 1000 tttn : full displacement` \<close>
-    else if unsigned_bitfield_extract_u8 4 4 op = 0b1000 then
-      let flag = (unsigned_bitfield_extract_u8 0 4 op) in
+    else if bitfield_extract 4 4 op = 0b1000 then
+      let flag = (bitfield_extract 0 4 op) in
       case nth_error l_bin (pc+2) of None \<Rightarrow> None | Some i1 \<Rightarrow> (
       case nth_error l_bin (pc+3) of None \<Rightarrow> None | Some i2 \<Rightarrow> (
       case nth_error l_bin (pc+4) of None \<Rightarrow> None | Some i3 \<Rightarrow> (
@@ -145,15 +145,15 @@ definition x64_decode_op_not_rex :: "u8 \<Rightarrow> nat \<Rightarrow> x64_bin 
 "x64_decode_op_not_rex h pc l_bin = (
     \<comment> \<open> R1 [opcode] \<close>
     \<comment> \<open> P2885 `PUSH: qwordregister (alternate encoding)`   -> ` 0100 W00BS : 0101 0 reg64` \<close>
-  if unsigned_bitfield_extract_u8 3 5 h = 0b01010 then
-    let reg2 = unsigned_bitfield_extract_u8 0 3 h in
-    let dst  = bitfield_insert_u8 3 1 reg2 0 in
+  if bitfield_extract 3 5 h = 0b01010 then
+    let reg2 = bitfield_extract 0 3 h in
+    let dst  = bitfield_insert 3 1 reg2 0 in
     case ireg_of_u8 dst of None \<Rightarrow> None | Some dst \<Rightarrow> (
     Some (1, Ppushl_r dst))
     \<comment> \<open> P2885 `POP: qwordregister (alternate encoding)`   -> ` 0100 W00B : 0101 1 reg64 ` \<close>
-    else if unsigned_bitfield_extract_u8 3 5 h = 0b01011 then
-    let reg2 = unsigned_bitfield_extract_u8 0 3 h in
-    let dst  = bitfield_insert_u8 3 1 reg2 0 in
+    else if bitfield_extract 3 5 h = 0b01011 then
+    let reg2 = bitfield_extract 0 3 h in
+    let dst  = bitfield_insert 3 1 reg2 0 in
     case ireg_of_u8 dst of None \<Rightarrow> None | Some dst \<Rightarrow> (
     Some (1, Ppopl dst))
     \<comment> \<open> R4 [opcode + displacement] \<close>
@@ -175,11 +175,11 @@ definition x64_decode_op_not_rex :: "u8 \<Rightarrow> nat \<Rightarrow> x64_bin 
       Some d \<Rightarrow> ( Some (5, Pjmp (scast d))) ))))
     else
     case nth_error l_bin (pc+1) of None \<Rightarrow> None | Some reg \<Rightarrow>
-    let modrm = unsigned_bitfield_extract_u8 6 2 reg in
-    let reg1  = unsigned_bitfield_extract_u8 3 3 reg in
-    let reg2  = unsigned_bitfield_extract_u8 0 3 reg in
-    let src   = bitfield_insert_u8 3 1 reg1 0 in
-    let dst   = bitfield_insert_u8 3 1 reg2 0 in
+    let modrm = bitfield_extract 6 2 reg in
+    let reg1  = bitfield_extract 3 3 reg in
+    let reg2  = bitfield_extract 0 3 reg in
+    let src   = bitfield_insert 3 1 reg1 0 in
+    let dst   = bitfield_insert 3 1 reg2 0 in
     \<comment> \<open> R2 [opcode + modrm] \<close>
     if h = 0x89 then 
     \<comment> \<open> P2887 `MOV register1 to register2` -> `0100 0R0B : 1000 1001 : 11 reg1 reg2` \<close>
@@ -436,11 +436,11 @@ definition x64_decode_op_0x81 :: "u8 \<Rightarrow> u8 \<Rightarrow> u8 \<Rightar
           else None)) ))))
   else if modrm = 0b10 \<and> reg2 = 0b100 then
     case nth_error l_bin (pc+3) of None \<Rightarrow> None | Some sib \<Rightarrow> (
-    let rbase  = unsigned_bitfield_extract_u8 0 3 sib in
-    let rindex = unsigned_bitfield_extract_u8 3 3 sib in
-    let scale  = unsigned_bitfield_extract_u8 6 2 sib in
-    let index  = bitfield_insert_u8 3 1 rindex x in
-    let base   = bitfield_insert_u8 3 1 rbase  b in
+    let rbase  = bitfield_extract 0 3 sib in
+    let rindex = bitfield_extract 3 3 sib in
+    let scale  = bitfield_extract 6 2 sib in
+    let index  = bitfield_insert 3 1 rindex x in
+    let base   = bitfield_insert 3 1 rbase  b in
       case nth_error l_bin (pc+4) of None \<Rightarrow> None | Some d1 \<Rightarrow> (
       case nth_error l_bin (pc+5) of None \<Rightarrow> None | Some d2 \<Rightarrow> (
       case nth_error l_bin (pc+6) of None \<Rightarrow> None | Some d3 \<Rightarrow> (
@@ -477,15 +477,15 @@ definition x64_decode :: "nat \<Rightarrow> x64_bin \<Rightarrow> (nat * instruc
       x64_decode_op_0x66 pc l_bin
     else if h = 0x0f then \<comment> \<open> R8 escape \<close>
       x64_decode_op_0x0f pc l_bin
-    else if unsigned_bitfield_extract_u8 4 4 h \<noteq> 0b0100 then  \<comment> \<open> h is not rex  \<close>
+    else if bitfield_extract 4 4 h \<noteq> 0b0100 then  \<comment> \<open> h is not rex  \<close>
         x64_decode_op_not_rex h pc l_bin
-    else if unsigned_bitfield_extract_u8 0 4 h = 0 then   \<comment> \<open> h is rex, the low 4-bit must not 0  \<close> 
+    else if bitfield_extract 0 4 h = 0 then   \<comment> \<open> h is rex, the low 4-bit must not 0  \<close> 
       None
     else  \<comment> \<open> h is rex  \<close> 
-      let w = unsigned_bitfield_extract_u8 3 1 h in
-      let r = unsigned_bitfield_extract_u8 2 1 h in
-      let x = unsigned_bitfield_extract_u8 1 1 h in
-      let b = unsigned_bitfield_extract_u8 0 1 h in (
+      let w = bitfield_extract 3 1 h in
+      let r = bitfield_extract 2 1 h in
+      let x = bitfield_extract 1 1 h in
+      let b = bitfield_extract 0 1 h in (
       case nth_error l_bin (pc+1) of None \<Rightarrow> None | Some op \<Rightarrow>
       \<comment> \<open> R6.1 [rex + opcode] \<close>
       if op = 0x99 then
@@ -493,26 +493,26 @@ definition x64_decode :: "nat \<Rightarrow> x64_bin \<Rightarrow> (nat * instruc
           Some (2, Pcqo)
         else None
       \<comment> \<open> P2885 `PUSH: qwordregister (alternate encoding)`   -> ` 0100 W00BS : 0101 0 reg64` \<close>
-      else if unsigned_bitfield_extract_u8 3 5 op = 0b01010 then
-        let reg2 = unsigned_bitfield_extract_u8 0 3 op in
-        let dst  = bitfield_insert_u8 3 1 reg2 b in
+      else if bitfield_extract 3 5 op = 0b01010 then
+        let reg2 = bitfield_extract 0 3 op in
+        let dst  = bitfield_insert 3 1 reg2 b in
         case ireg_of_u8 dst of None \<Rightarrow> None | Some dst \<Rightarrow> (
           if w = 0 \<and> r = 0 \<and> x = 0 then
             Some (2, Ppushl_r dst)
           else None)
       \<comment> \<open> P2885 `POP: qwordregister (alternate encoding)`   -> ` 0100 W00B : 0101 1 reg64 ` \<close>
-      else if unsigned_bitfield_extract_u8 3 5 op = 0b01011 then
-        let reg2 = unsigned_bitfield_extract_u8 0 3 op in
-        let dst  = bitfield_insert_u8 3 1 reg2 b in
+      else if bitfield_extract 3 5 op = 0b01011 then
+        let reg2 = bitfield_extract 0 3 op in
+        let dst  = bitfield_insert 3 1 reg2 b in
         case ireg_of_u8 dst of None \<Rightarrow> None | Some dst \<Rightarrow> (
           if w = 0 \<and> r = 0 \<and> x = 0 then
             Some (2, Ppopl dst)
           else None)
       \<comment> \<open> R6.2 [rex + opcode + imm] \<close> 
       \<comment> \<open> P2882 `MOV immediate64 to qwordregister (alternate encoding)` -> `0100 100B 1011 1reg : imm64` \<close>
-      else if unsigned_bitfield_extract_u8 3 5 op = 0b10111 then
-        let reg2 = unsigned_bitfield_extract_u8 0 3 op in
-        let dst  = bitfield_insert_u8 3 1 reg2 b in
+      else if bitfield_extract 3 5 op = 0b10111 then
+        let reg2 = bitfield_extract 0 3 op in
+        let dst  = bitfield_insert 3 1 reg2 b in
         case nth_error l_bin (pc+2) of None \<Rightarrow> None | Some i1 \<Rightarrow> (
         case nth_error l_bin (pc+3) of None \<Rightarrow> None | Some i2 \<Rightarrow> (
         case nth_error l_bin (pc+4) of None \<Rightarrow> None | Some i3 \<Rightarrow> (
@@ -543,9 +543,9 @@ definition x64_decode :: "nat \<Rightarrow> x64_bin \<Rightarrow> (nat * instruc
       \<comment> \<open> R8.4 [rex + escape + opcode] \<close>
       \<comment> \<open> P2877 `BSWAP: register `   -> `0000 1111 : 1100 1 reg` \<close>
       \<comment> \<open> P2877 `BSWAP: qwordregister `   -> `0100 100B 0000 1111 : 1100 1 reg` \<close>
-      if unsigned_bitfield_extract_u8 3 5 op1 = 0b11001 then
-        let reg2 = unsigned_bitfield_extract_u8 0 3 op1 in
-        let dst  = bitfield_insert_u8 3 1 reg2 b in
+      if bitfield_extract 3 5 op1 = 0b11001 then
+        let reg2 = bitfield_extract 0 3 op1 in
+        let dst  = bitfield_insert 3 1 reg2 b in
           case ireg_of_u8 dst of None \<Rightarrow> None | Some dst \<Rightarrow> (
             if w = 1 \<and> x = 0 \<and> r = 0 then
               Some (3, Pbswapq dst)
@@ -555,14 +555,14 @@ definition x64_decode :: "nat \<Rightarrow> x64_bin \<Rightarrow> (nat * instruc
       \<comment> \<open> R8.5 [rex + escape + opcode + modrm] \<close>
       \<comment> \<open> P2919 `MOVcc : resgister2  to resgister1 ` -> `0100 0R0B 0000 1111: 0100 tttn : 11 reg1 reg2` \<close>
       \<comment> \<open> P2919 `MOVcc : qwordregister2 to qwordregister1` -> ` 0100 1R0B 0000 1111: 0100 tttn : 11 qwordreg1 qwordreg2` \<close>
-        else if unsigned_bitfield_extract_u8 4 4 op1 = 0b0100 then
-          let flag = (unsigned_bitfield_extract_u8 0 4 op1)  in 
+        else if bitfield_extract 4 4 op1 = 0b0100 then
+          let flag = (bitfield_extract 0 4 op1)  in 
           case nth_error l_bin (pc+3) of None \<Rightarrow> None | Some reg \<Rightarrow>
-          let modrm = unsigned_bitfield_extract_u8 6 2 reg in
-          let reg1  = unsigned_bitfield_extract_u8 3 3 reg in
-          let reg2  = unsigned_bitfield_extract_u8 0 3 reg in
-          let src   = bitfield_insert_u8 3 1 reg1 r in
-          let dst   = bitfield_insert_u8 3 1 reg2 b in
+          let modrm = bitfield_extract 6 2 reg in
+          let reg1  = bitfield_extract 3 3 reg in
+          let reg2  = bitfield_extract 0 3 reg in
+          let src   = bitfield_insert 3 1 reg1 r in
+          let dst   = bitfield_insert 3 1 reg2 b in
             if modrm = 0b11 then
               case cond_of_u8 flag of None \<Rightarrow> None | Some t \<Rightarrow>(
               case ireg_of_u8 src of None \<Rightarrow> None | Some src \<Rightarrow> (
@@ -576,11 +576,11 @@ definition x64_decode :: "nat \<Rightarrow> x64_bin \<Rightarrow> (nat * instruc
         else None
       else (
         case nth_error l_bin (pc+2) of None \<Rightarrow> None | Some reg \<Rightarrow>
-        let modrm = unsigned_bitfield_extract_u8 6 2 reg in
-        let reg1  = unsigned_bitfield_extract_u8 3 3 reg in
-        let reg2  = unsigned_bitfield_extract_u8 0 3 reg in
-        let src   = bitfield_insert_u8 3 1 reg1 r in
-        let dst   = bitfield_insert_u8 3 1 reg2 b in
+        let modrm = bitfield_extract 6 2 reg in
+        let reg1  = bitfield_extract 3 3 reg in
+        let reg2  = bitfield_extract 0 3 reg in
+        let src   = bitfield_insert 3 1 reg1 r in
+        let dst   = bitfield_insert 3 1 reg2 b in
           \<comment> \<open> R6.3 [rex + opcode + modrm] \<close>
           if op = 0x89 then
             if modrm = 0b11 then (
@@ -617,11 +617,11 @@ definition x64_decode :: "nat \<Rightarrow> x64_bin \<Rightarrow> (nat * instruc
                       Some (7, Pmov_mr (Addrmode (Some rb) None dis) src (if w = 1 then M64 else M32))))) ))))
               else 
                 case nth_error l_bin (pc+3) of None \<Rightarrow> None | Some sib \<Rightarrow> (
-                let rbase  = unsigned_bitfield_extract_u8 0 3 sib in
-                let rindex = unsigned_bitfield_extract_u8 3 3 sib in
-                let scale  = unsigned_bitfield_extract_u8 6 2 sib in
-                let index  = bitfield_insert_u8 3 1 rindex x in
-                let base   = bitfield_insert_u8 3 1 rbase  b in
+                let rbase  = bitfield_extract 0 3 sib in
+                let rindex = bitfield_extract 3 3 sib in
+                let scale  = bitfield_extract 6 2 sib in
+                let index  = bitfield_insert 3 1 rindex x in
+                let base   = bitfield_insert 3 1 rbase  b in
                 case nth_error l_bin (pc+4) of None \<Rightarrow> None | Some d1 \<Rightarrow> (
                 case nth_error l_bin (pc+5) of None \<Rightarrow> None | Some d2 \<Rightarrow> (
                 case nth_error l_bin (pc+6) of None \<Rightarrow> None | Some d3 \<Rightarrow> (
@@ -646,11 +646,11 @@ definition x64_decode :: "nat \<Rightarrow> x64_bin \<Rightarrow> (nat * instruc
           else if modrm = 0b10 then 
             if reg2 = 0b100 then
               case nth_error l_bin (pc+3) of None \<Rightarrow> None | Some sib \<Rightarrow> (
-              let rbase  = unsigned_bitfield_extract_u8 0 3 sib in
-              let rindex = unsigned_bitfield_extract_u8 3 3 sib in
-              let scale  = unsigned_bitfield_extract_u8 6 2 sib in
-              let index  = bitfield_insert_u8 3 1 rindex x in
-              let base   = bitfield_insert_u8 3 1 rbase  b in
+              let rbase  = bitfield_extract 0 3 sib in
+              let rindex = bitfield_extract 3 3 sib in
+              let scale  = bitfield_extract 6 2 sib in
+              let index  = bitfield_insert 3 1 rindex x in
+              let base   = bitfield_insert 3 1 rbase  b in
                 case nth_error l_bin (pc+4) of None \<Rightarrow> None | Some d1 \<Rightarrow> (
                 case nth_error l_bin (pc+5) of None \<Rightarrow> None | Some d2 \<Rightarrow> (
                 case nth_error l_bin (pc+6) of None \<Rightarrow> None | Some d3 \<Rightarrow> (
@@ -854,11 +854,11 @@ definition x64_decode :: "nat \<Rightarrow> x64_bin \<Rightarrow> (nat * instruc
         \<comment> \<open> P2885 `PUSH: memory64`   -> `0100 W00BS : 1111 1111 : mod 110 r/m ` \<close>
           else if modrm = 0b10 \<and> reg2 = 0b100 then                           
             case nth_error l_bin (pc+3) of None \<Rightarrow> None | Some sib \<Rightarrow> (
-            let rbase  = unsigned_bitfield_extract_u8 0 3 sib in
-            let rindex = unsigned_bitfield_extract_u8 3 3 sib in
-            let scale  = unsigned_bitfield_extract_u8 6 2 sib in
-            let index  = bitfield_insert_u8 3 1 rindex x in
-            let base   = bitfield_insert_u8 3 1 rbase  b in
+            let rbase  = bitfield_extract 0 3 sib in
+            let rindex = bitfield_extract 3 3 sib in
+            let scale  = bitfield_extract 6 2 sib in
+            let index  = bitfield_insert 3 1 rindex x in
+            let base   = bitfield_insert 3 1 rbase  b in
               case nth_error l_bin (pc+4) of None \<Rightarrow> None | Some d1 \<Rightarrow> (
               case nth_error l_bin (pc+5) of None \<Rightarrow> None | Some d2 \<Rightarrow> (
               case nth_error l_bin (pc+6) of None \<Rightarrow> None | Some d3 \<Rightarrow> (
@@ -964,11 +964,11 @@ definition x64_decode :: "nat \<Rightarrow> x64_bin \<Rightarrow> (nat * instruc
                 else None)))  ))))
             else \<comment> \<open> sib \<close>
               case nth_error l_bin (pc+3) of None \<Rightarrow> None | Some sib \<Rightarrow> (
-              let rbase  = unsigned_bitfield_extract_u8 0 3 sib in
-              let rindex = unsigned_bitfield_extract_u8 3 3 sib in
-              let scale  = unsigned_bitfield_extract_u8 6 2 sib in
-              let index  = bitfield_insert_u8 3 1 rindex x in
-              let base   = bitfield_insert_u8 3 1 rbase  b in
+              let rbase  = bitfield_extract 0 3 sib in
+              let rindex = bitfield_extract 3 3 sib in
+              let scale  = bitfield_extract 6 2 sib in
+              let index  = bitfield_insert 3 1 rindex x in
+              let base   = bitfield_insert 3 1 rbase  b in
                 case nth_error l_bin (pc+4) of None \<Rightarrow> None | Some d1 \<Rightarrow> (
                 case nth_error l_bin (pc+5) of None \<Rightarrow> None | Some d2 \<Rightarrow> (
                 case nth_error l_bin (pc+6) of None \<Rightarrow> None | Some d3 \<Rightarrow> (
@@ -1032,13 +1032,13 @@ value "x64_disassemble [102, 65, 137, 200]"
 value "102 = (0x66::u8)"
 value "137 = (0x89::u8)"
 
-value "unsigned_bitfield_extract_u8 2 1 64" (**r r = 0 *)
-value "unsigned_bitfield_extract_u8 0 1 64" (**r b = 0 *)
-value "unsigned_bitfield_extract_u8 6 2 195" (**r modrm = 3 *)
-value "unsigned_bitfield_extract_u8 3 3 200" (**r reg1 = 0 *)
-value "unsigned_bitfield_extract_u8 0 3 195" (**r reg2 = 3 *)
-value "bitfield_insert_u8 3 1 0 0" (**r src = 0 *)
-value "bitfield_insert_u8 3 1  3 0" (**r dst = 3 *)
+value "bitfield_extract 2 1 64" (**r r = 0 *)
+value "bitfield_extract 0 1 64" (**r b = 0 *)
+value "bitfield_extract 6 2 195" (**r modrm = 3 *)
+value "bitfield_extract 3 3 200" (**r reg1 = 0 *)
+value "bitfield_extract 0 3 195" (**r reg2 = 3 *)
+value "bitfield_insert 3 1 0 0" (**r src = 0 *)
+value "bitfield_insert 3 1  3 0" (**r dst = 3 *)
 value "ireg_of_u8 0" (**r Some RAX *)
 value "ireg_of_u8 3" (**r Some RBX *) *)
 
