theory/BitExtractInsert.thy
@@ -1,0 +1,171 @@
+theory BitExtractInsert
+  imports Main rBPFCommType
+begin
+
+lemma and_pow_n_shr_eq: "(and (x::'a :: len word) (2^n) = 0) = (and 1 (x >> n) = 0)"
+  apply (induction n arbitrary: x; simp)
+  subgoal for x
+    using and.commute
+    by metis
+  subgoal for n1 x
+    apply (cases "even x"; simp?)
+    subgoal
+      by (metis and_exp_eq_0_iff_not_bit bit_0 bit_iff_odd_drop_bit power_0 power_Suc word_bw_comms(1))
+    subgoal
+      by (metis and_exp_eq_0_iff_not_bit even_drop_bit_iff_not_bit even_iff_mod_2_eq_zero one_and_eq power_Suc)
+    done
+  done
+
+lemma word_and_le_2: "and x y = z \<Longrightarrow> (y :: 'a :: len word) < z \<Longrightarrow> False"
+  using word_le_def AND_upper2'' word_and_le1
+  using leD by blast
+
+lemma and_length_eq: "and (2^LENGTH('a) -1) x = (x::'a :: len word)"
+  by simp
+
+lemma and_length_eq_u8: "and 255 x = (x::8 word)"
+  apply (subgoal_tac "2^LENGTH(8)-1 = (255::u8)")
+  subgoal using and_length_eq
+    by metis 
+  subgoal by simp
+  done
+
+lemma bitfield_extract_0_8_eq: "bitfield_extract 0 8 x = (x::u8)"
+  by (simp add: bitfield_extract_def Let_def and_length_eq_u8)
+
+lemma bit_power_k_add_m_low: "bit (2 ^ (m + n) - 2 ^ n) k \<Longrightarrow> n \<le> k"
+  apply (induction n arbitrary: m k; simp)
+  subgoal for n1 m k
+    apply (cases k; simp)
+    subgoal
+      by (metis bit_double_iff right_diff_distrib')
+    subgoal for k1
+      by (metis bit_double_Suc_iff right_diff_distrib')
+    done
+  done
+
+lemma bit_power_k_minus_1_lt: "k \<le> LENGTH('a) \<Longrightarrow> bit ((2^k -1)::'a :: len word) n \<longleftrightarrow> n < k"
+  apply (simp only: bit_iff_odd)
+  using even_decr_exp_div_exp_iff' linorder_not_le
+  using even_mask_div_iff by fastforce
+
+lemma bit_power_k_add_m_high: "m + n \<le> LENGTH('a) \<Longrightarrow> bit ((2 ^ (m + n) - 2 ^ n)::'a :: len word) k \<Longrightarrow> k < m + n"
+  apply (induction n arbitrary: m k; simp)
+  subgoal for m k using bit_power_k_minus_1_lt by blast
+  subgoal for n1 m k
+    apply (cases k; simp)
+    subgoal
+      by (metis One_nat_def Suc_leD bit_double_iff diff_Suc_1' right_diff_distrib')
+    done
+  done
+
+lemma bit_power_k_add_m_iff: "m + n \<le> LENGTH('a) \<Longrightarrow> bit ((2 ^ (m + n) - 2 ^ n)::'a :: len word) k = (n \<le> k \<and> k < m + n)"
+  apply (induction n arbitrary: m k; simp)
+  subgoal for m k using bit_power_k_minus_1_lt by blast
+  subgoal for n1 m k
+    apply (cases k; simp)
+    subgoal
+      by (metis bit_double_iff right_diff_distrib')
+    subgoal for k1
+      by (metis (no_types, lifting) add_leD2 bit_double_Suc_iff nat_add_left_cancel_less order_less_le_trans plus_1_eq_Suc possible_bit_word right_diff_distrib_numeral)
+    done
+  done
+
+
+lemma and_power_m_add_n_shift_n_eq: "m + n \<le> LENGTH('a) \<Longrightarrow> and (2^(m+n) - 2^n) ((x >> n) << n) =
+  and (2^(m+n) - 2^n) (x::'a :: len word)"
+  apply (simp add: bit_eq_iff)
+  apply (simp add: bit_simps)
+  apply (rule allI)
+  subgoal for n1
+    apply (cases "n \<le> n1"; simp)
+    apply (rule impI)
+    apply (simp add: bit_power_k_add_m_low)
+    done
+  done
+
+
+lemma and_shr_shl_eq: "and (2^LENGTH('a) - 2^n) ((x >> n) << n) =
+  and (2^LENGTH('a) - 2^n) (x::'a :: len word)"
+  apply (simp add: bit_eq_iff)
+  apply (simp add: bit_simps)
+  by (metis add_diff_inverse_nat bit_iff_odd even_mask_div_iff exp_eq_0_imp_not_bit linorder_not_le)
+
+lemma and_shr_shl_eq_u8_6: "(and 192 ((x >> 6) << 6)) = and 192 (x:: 8 word)"
+  apply (subgoal_tac "2^LENGTH(8) - 2^6 = (192::u8)")
+  subgoal using and_shr_shl_eq
+    by metis
+
+  subgoal by simp
+  done
+
+
+lemma pow_2_m1_shl_eq: "m + n \<le> LENGTH('a) \<Longrightarrow> 2 ^ n - 1 << m = 2^(m+n) - (2^m ::'a :: len word)"
+  apply (induction m arbitrary: n; simp)
+  subgoal for m1 n
+    apply (simp only: Nat.add_Suc_right[symmetric])
+    apply (subgoal_tac"2 ^ n * 2 = (2 ^ (Suc n) ::'a :: len word)")
+     prefer 2 subgoal by simp
+    by (simp add: mult.commute power_add push_bit_eq_mult right_diff_distrib')
+  done
+
+lemma bitfield_extract_split_eq :"
+  m + n \<le> LENGTH('a) \<Longrightarrow>
+  bitfield_extract 0 m r = x \<Longrightarrow>
+  bitfield_extract m n r = v \<Longrightarrow>
+    bitfield_insert m n x v = bitfield_extract 0 (m+n) (r::'a :: len word)"
+  apply (erule subst [of _ v])
+  apply (erule subst [of _ x])
+  apply (simp add: bitfield_insert_def bitfield_extract_def Let_def)
+  apply (simp only: pow_2_m1_shl_eq)
+  apply (simp only: add.commute [of m n])
+  apply (simp add: and_power_m_add_n_shift_n_eq)
+  apply (simp add: bit_eq_iff bit_simps)
+
+  apply (rule allI, rule impI)
+  subgoal for n1
+    apply (cases "bit r n1"; simp)
+    apply (cases "m \<le> n1"; simp?)
+    prefer 2
+    subgoal 
+      by (simp add: bit_power_k_minus_1_lt)
+
+    apply (subgoal_tac "bit ((2 ^ m - 1)::'a :: len word) n1 = False"; simp)
+     prefer 2 subgoal
+      using bit_iff_odd even_mask_div_iff by blast
+    apply (cases "n+m \<le> n1"; simp add: bit_power_k_add_m_iff)
+    prefer 2
+    subgoal
+      using bit_power_k_minus_1_lt [of "n+m" n1]
+      using linorder_not_le by blast
+    subgoal
+      using bit_iff_odd even_mask_div_iff by blast
+    done
+  done
+named_theorems extract_simp
+
+lemma bitfield_extract_0_6_2_eq [extract_simp] :"
+  bitfield_extract 0 6 r = x \<Longrightarrow>
+  bitfield_extract 6 2 r = v \<Longrightarrow>
+    bitfield_insert 6 2 x v = (r::u8)"
+  apply (simp add: bitfield_extract_split_eq)
+  apply (simp add: bitfield_extract_0_8_eq)
+  done
+
+lemma bitfield_extract_0_3_3_eq :"
+  bitfield_extract 0 3 r = x \<Longrightarrow>
+  bitfield_extract 3 3 r = v \<Longrightarrow>
+    bitfield_insert 3 3 x v = bitfield_extract 0 6 (r::u8)"
+  apply (simp add: bitfield_extract_split_eq)
+  done
+
+lemma "m + n \<le> LENGTH('a) \<Longrightarrow>
+  (2 ^ n - 1 << m) >> m = ((2 ^ n - 1)::'a :: len word)"
+
+lemma "
+  m + n \<le> LENGTH('a) \<Longrightarrow>
+  bitfield_extract m n (bitfield_insert m n k v) =
+  bitfield_extract 0 n (v::'a :: len word)"
+  apply (simp add: bitfield_extract_def bitfield_insert_def)
+
+end
