theory/x64EncodeProof.thy
@@ -1,7 +1,7 @@
  theory x64EncodeProof
 imports
   Main
-  rBPFCommType
+  rBPFCommType BitExtractInsert
   x64Assembler x64Disassembler
 (*  x64_encode_movl_rr_1 x64_encode_movl_rr_3  x64_encode_movl_rr_4
   x64_encode_movq_rr_1
@@ -15,85 +15,36 @@ imports
   x64_encode_subl_ri_1 x64_encode_subl_ri_2   x64_encode_movl_ri_3*)
 begin
 
-lemma u8_of_ireg_of_u8_implies: "(ireg_of_u8 i = Some r) \<Longrightarrow> (u8_of_ireg r = i)"
-  using u8_of_ireg_of_u8_iff by blast
 
-lemma word_and_le_2: "and x y = z \<Longrightarrow> (y :: 'a :: len word) < z \<Longrightarrow> False"
-  using word_le_def AND_upper2'' word_and_le1
-  using leD by blast
-
-lemma bitfield_insert_u8_3_1_0: "ireg_of_u8 (bitfield_insert_u8 3 1 n 0) = Some dst \<Longrightarrow>
-    and (u8_of_ireg dst) 8 = 0"
-  apply (drule u8_of_ireg_of_u8_implies, simp)
-  apply (simp add: bitfield_insert_u8_def unsigned_bitfield_extract_u8_def ireg_of_u8_def split: if_split_asm)
-  apply (simp add: and.assoc)
-  done
-
-lemma and_length_eq: "and (2^LENGTH('a) -1) x = (x::'a :: len word)"
-  by simp
-
-lemma and_length_eq_u8: "and 255 x = (x::8 word)"
-  apply (subgoal_tac "2^LENGTH(8)-1 = (255::u8)")
-  subgoal using and_length_eq
-    by metis 
-  subgoal by simp
-  done
-
-lemma unsigned_bitfield_extract_u8_0_8_eq: "unsigned_bitfield_extract_u8 0 8 x = (x::u8)"
-  by (simp add: unsigned_bitfield_extract_u8_def Let_def and_length_eq_u8)
-
-
-lemma and_shr_shl_eq: "and ((2^LENGTH('a) -1) - (2^n -1)) ((x >> n) << n) =
-  and ((2^LENGTH('a) -1) - (2^n -1)) (x::'a :: len word)"
-  apply (simp add: bit_eq_iff)
-  apply (simp add: bit_simps)
-  by (metis add_diff_inverse_nat bit_iff_odd even_mask_div_iff exp_eq_0_imp_not_bit linorder_not_le)
-
-lemma and_shr_shl_eq_u8_6: "(and 192 ((x >> 6) << 6)) = and 192 (x:: 8 word)"
-  apply (subgoal_tac "(2^LENGTH(8) -1) - (2^6 -1) = (192::u8)")
-  subgoal using and_shr_shl_eq
-    by metis
-
-  subgoal by simp
-  done
-
-lemma unsigned_bitfield_extract_u8_split_eq :"
-  m+n = 8 \<Longrightarrow>
-  unsigned_bitfield_extract_u8 0 m r = x \<Longrightarrow>
-  unsigned_bitfield_extract_u8 m n r = v \<Longrightarrow>
-    bitfield_insert_u8 m n x v = (r::u8)"
-  apply (erule subst [of _ v])
-  apply (erule subst [of _ x])
-  apply (simp add: bitfield_insert_u8_def unsigned_bitfield_extract_u8_def Let_def)
-
-lemma unsigned_bitfield_extract_u8_0_6_2_eq :"
-  unsigned_bitfield_extract_u8 0 6 r = x \<Longrightarrow>
-  unsigned_bitfield_extract_u8 6 2 r = v \<Longrightarrow>
-    bitfield_insert_u8 6 2 x v = (r::u8)"
-  apply (erule subst [of _ v])
-  apply (erule subst [of _ x])
-  apply (simp add: bitfield_insert_u8_def unsigned_bitfield_extract_u8_def Let_def)
-  apply (simp add: and_shr_shl_eq_u8_6)
-  apply (simp add: and.commute [of _ "- 193"] and.assoc[symmetric])
-  sorry
 
 
 (*
-lemma bitfield_insert_u8_3_1_1: "ireg_of_u8 (bitfield_insert_u8 3 1 n 1) = Some dst \<Longrightarrow>
+lemma bitfield_insert_3_1_1: "ireg_of_u8 (bitfield_insert 3 1 n 1) = Some dst \<Longrightarrow>
     and (u8_of_ireg dst) 8 = 1"
   apply (drule u8_of_ireg_of_u8_implies, simp)
-  apply (simp add: bitfield_insert_u8_def unsigned_bitfield_extract_u8_def ireg_of_u8_def split: if_split_asm)
+  apply (simp add: bitfield_insert_def bitfield_extract_def ireg_of_u8_def split: if_split_asm)
   apply (simp add: and.assoc)
   done *)
-find_theorems "and 7 _"
+
+
+lemma and_8_neq_0_eq [extract_simp]: "(and x 8\<noteq>0) = (bitfield_extract 3 1 (x:: u8)\<noteq>0)"
+  apply (simp add: bitfield_extract_def)
+  apply (subgoal_tac "(8::u8) = 2^3")
+  prefer 2 subgoal by simp
+  using and_pow_n_shr_eq [of x 3]
+  by simp
+
 lemma "
-  unsigned_bitfield_extract_u8 6 2 reg = 3 \<Longrightarrow>
-  bitfield_insert_u8 3 (Suc 0) (unsigned_bitfield_extract_u8 3 3 reg) 0 = 0 \<Longrightarrow>
-  ireg_of_u8 (bitfield_insert_u8 3 (Suc 0) (unsigned_bitfield_extract_u8 0 3 reg) 0) = Some dst \<Longrightarrow>
+  bitfield_extract 6 2 reg = 3 \<Longrightarrow>
+  bitfield_insert 3 (Suc 0) (bitfield_extract 3 3 reg) 0 = 0 \<Longrightarrow>
+  ireg_of_u8 (bitfield_insert 3 (Suc 0) (bitfield_extract 0 3 reg) 0) = Some dst \<Longrightarrow>
   construct_rex_to_u8 False False False (and (u8_of_ireg dst) 8 \<noteq> 0) = 64 
      \<Longrightarrow> construct_modsib_to_u8 3 0 (u8_of_ireg dst) = reg"
   apply (drule u8_of_ireg_of_u8_implies, simp add: construct_modsib_to_u8_def)
-  apply (rule unsigned_bitfield_extract_u8_0_6_2_eq; simp?)
+  apply (rule extract_simp; simp?)
+  apply (simp add: extract_simp)
+  apply (rule bitfield_extract_0_3_3_eq; simp?)
+  apply (simp add: bitfield_extract_split_eq [of 3 3]) 
 
 
 
@@ -109,8 +60,8 @@ declare x64_decode_op_0x81_def [simp]
 
 lemma x64_decode_encode_consistency:
   "list_in_list l_bin pc l \<Longrightarrow> x64_decode pc l = Some (length l_bin, ins) \<Longrightarrow>  Some l_bin = x64_encode ins"
-  apply (unfold x64_decode_def)
-
+  apply (simp add: x64_decode_def)
+                     
   apply (cases "nth_error l pc"; simp)
   subgoal for h
     by (cases l_bin; simp)
@@ -128,7 +79,7 @@ lemma x64_decode_encode_consistency:
       subgoal for reg
         apply (cases "nth_error l (pc + 3)"; simp)
         subgoal for imm
-          apply (cases "ireg_of_u8 (bitfield_insert_u8 3 (Suc 0) (unsigned_bitfield_extract_u8 0 3 reg) 0)"; simp)
+          apply (cases "ireg_of_u8 (bitfield_insert 3 (Suc 0) (bitfield_extract 0 3 reg) 0)"; simp)
           subgoal for dst
             apply (erule conjE)
             apply (drule sym[of _ ins], simp)
@@ -170,7 +121,7 @@ Proof done
         done
       done
 
-    subgoal by (unfold bitfield_insert_u8_def;simp)
+    subgoal by (unfold bitfield_insert_def;simp)
 
     subgoal 
       apply (cases l_bin, simp_all)
@@ -310,7 +261,7 @@ Proof done
         done
       done
 
-    subgoal by (unfold bitfield_insert_u8_def;simp)
+    subgoal by (unfold bitfield_insert_def;simp)
 
     subgoal 
       apply (cases l_bin, simp_all)
@@ -515,7 +466,7 @@ Proof done
         done
       done
 
-    subgoal by (unfold bitfield_insert_u8_def;simp)
+    subgoal by (unfold bitfield_insert_def;simp)
 
     subgoal 
       apply (cases l_bin, simp_all)
@@ -636,7 +587,7 @@ Proof done
 
     subgoal
       apply (simp add: u8_of_ireg_of_u8_iff[symmetric])
-      apply (unfold bitfield_insert_u8_def u8_of_bool_def Let_def)
+      apply (unfold bitfield_insert_def u8_of_bool_def Let_def)
       apply simp
       done
 
